ProofLibrary.lean
@@ -1,3 +1,4 @@
+import ProofLibrary.AlternativeMatches
 import ProofLibrary.ChaseSequence.Basic
 import ProofLibrary.ChaseSequence.Universality
 import ProofLibrary.ChaseSequence.Deterministic
