ProofLibrary/AlternativeMatches.lean
@@ -1,0 +1,60 @@
+import ProofLibrary.SubstitutionAndHomomorphismBasics
+import ProofLibrary.Trigger
+
+variable {sig : Signature} [DecidableEq sig.P] [DecidableEq sig.C] [DecidableEq sig.V]
+
+namespace GroundTermMapping
+
+  def isAlternativeMatch (h_alt : GroundTermMapping sig) (trg : PreTrigger sig) (disj_index : Fin trg.result.length) (fs : FactSet sig) : Prop :=
+    (h_alt.isHomomorphism (trg.result.get disj_index) fs) ∧
+    (∀ t, t ∈ trg.rule.frontier.map trg.subs -> h_alt t = t) ∧
+    (∃ n, (n ∈ (trg.result.get disj_index).terms) ∧ (¬ n ∈ (h_alt.applyFactSet (trg.result.get disj_index)).terms))
+
+end GroundTermMapping
+
+namespace PreTrigger
+
+  -- TODO: cleanup the proof; seems like we need lemmas on PreTrigger and Substitution Interaction (likely also useful elsewhere)
+  theorem satisfied_of_alternativeMatch (trg : PreTrigger sig) (fs : FactSet sig) : ∀ (h_alt : GroundTermMapping sig) (disj_index : Fin trg.result.length), h_alt.isAlternativeMatch trg disj_index fs -> trg.satisfied fs := by
+    intro h_alt disj_index is_alt_match
+    exists ⟨disj_index.val, by have isLt := disj_index.isLt; rw [PreTrigger.head_length_eq_mapped_head_length]; unfold PreTrigger.result at isLt; simp at isLt; exact isLt⟩
+    exists (h_alt ∘ trg.apply_to_var_or_const disj_index ∘ VarOrConst.var)
+    constructor
+    . intro v v_in_frontier
+      simp only [Function.comp_apply]
+      simp [PreTrigger.apply_to_var_or_const, PreTrigger.apply_to_skolemized_term, PreTrigger.skolemize_var_or_const, VarOrConst.skolemize, v_in_frontier]
+      apply is_alt_match.right.left
+      simp
+      exists v
+    . intro f f_mem
+      apply is_alt_match.left.right
+      rw [← List.inIffInToSet] at f_mem
+      unfold GroundSubstitution.apply_function_free_conj at f_mem
+      simp at f_mem
+      simp [PreTrigger.result, PreTrigger.mapped_head]
+      unfold GroundTermMapping.applyFactSet
+      rcases f_mem with ⟨a, a_mem, a_eq⟩
+      exists trg.apply_to_function_free_atom disj_index a
+      constructor
+      . rw [← List.inIffInToSet]
+        simp
+        exists a
+      . unfold PreTrigger.apply_to_function_free_atom
+        unfold GroundTermMapping.applyFact
+        simp
+        unfold GroundSubstitution.apply_function_free_atom at a_eq
+        rw [← a_eq]
+        simp [PreTrigger.apply_to_var_or_const]
+        intro t t_mem
+        unfold PreTrigger.apply_to_skolemized_term
+        unfold PreTrigger.skolemize_var_or_const
+        simp [GroundSubstitution.apply_var_or_const]
+        cases t with
+        | const c => simp [VarOrConst.skolemize, GroundSubstitution.apply_skolem_term]; apply is_alt_match.left.left (GroundTerm.const c)
+        | var v => simp
+
+  theorem alternativeMatch_of_satisfied (trg : PreTrigger sig) (fs : FactSet sig) (disj_index : Fin trg.result.length) (gt : GroundTerm sig) (gt_in_res_but_not_fs : gt ∈ (trg.result.get disj_index).terms ∧ ¬ gt ∈ fs.terms) : trg.satisfied_for_disj fs ⟨disj_index, sorry⟩ -> ∃ (h_alt : GroundTermMapping sig), h_alt.isAlternativeMatch trg disj_index fs := by
+    sorry
+
+end PreTrigger
+
